Rename triple to Triple; define Triple.and

MPL/Triple.lean
@@ -22,29 +22,32 @@ namespace MPL
 universe u
 variable {m : Type → Type u} {ps : PostShape} [WP m ps]
 
-def triple (x : m α) (P : Assertion ps) (Q : PostCond α ps) : Prop :=
+def Triple (x : m α) (P : Assertion ps) (Q : PostCond α ps) : Prop :=
   P ⊢ₛ wp⟦x⟧.apply Q
 
-notation:lead "⦃" P "⦄ " x:lead " ⦃" Q "⦄" => triple x spred(P) spred(Q)
-app_unexpand_rule triple
+notation:lead "⦃" P "⦄ " x:lead " ⦃" Q "⦄" => Triple x spred(P) spred(Q)
+app_unexpand_rule Triple
   | `($_ $x $P $Q) => match Q with
     | `(⇓ $xs* => $e) => do
       `(⦃$(← SPred.Notation.unpack P)⦄ $x ⦃⇓ $xs* => $(← SPred.Notation.unpack e)⦄)
     | _ => do
       `(⦃$(← SPred.Notation.unpack P)⦄ $x ⦃$(← SPred.Notation.unpack Q)⦄)
 
-instance [WP m ps] (x : m α) : ProofMode.PropAsEntails (triple x P Q) spred(P → wp⟦x⟧.apply Q) where
+instance [WP m ps] (x : m α) : ProofMode.PropAsEntails (Triple x P Q) spred(P → wp⟦x⟧.apply Q) where
   prop_as_entails := (SPred.entails_true_intro P (wp⟦x⟧.apply Q)).symm
 
-theorem triple_pure [Monad m] [MonadMorphism m (PredTrans ps) wp] {α} {Q : PostCond α ps} (a : α) (himp : P.entails (Q.1 a)) :
-  triple (pure (f:=m) a) P Q := himp.trans (by simp only [pure_pure, PredTrans.pure_apply, SPred.entails.refl])
+theorem Triple.pure [Monad m] [MonadMorphism m (PredTrans ps) wp] {α} {Q : PostCond α ps} (a : α) (himp : P.entails (Q.1 a)) :
+  Triple (pure (f:=m) a) P Q := himp.trans (by simp only [pure_pure, PredTrans.pure_apply, SPred.entails.refl])
 
-theorem triple_bind [Monad m] [MonadMorphism m (PredTrans ps) wp] {α β} {P : Assertion ps} {Q : α → Assertion ps} {R : PostCond β ps} (x : m α) (f : α → m β)
-  (hx : triple x P (Q, R.2))
-  (hf : ∀ b, triple (f b) (Q b) R) :
-  triple (x >>= f) P R := by
+theorem Triple.bind [Monad m] [MonadMorphism m (PredTrans ps) wp] {α β} {P : Assertion ps} {Q : α → Assertion ps} {R : PostCond β ps} (x : m α) (f : α → m β)
+  (hx : Triple x P (Q, R.2))
+  (hf : ∀ b, Triple (f b) (Q b) R) :
+  Triple (x >>= f) P R := by
     apply SPred.entails.trans hx
     simp only [bind_bind]
     apply wp⟦x⟧.mono _ _
     simp only [PostCond.entails, Assertion, FailConds.entails.refl, and_true]
     exact hf
+
+theorem Triple.and (x : m α) (h₁ : ⦃P₁⦄ x ⦃Q₁⦄) (h₂ : ⦃P₂⦄ x ⦃Q₂⦄) : ⦃P₁ ∧ P₂⦄ x ⦃Q₁ ∧ₚ Q₂⦄ :=
+  (SPred.and_mono h₁ h₂).trans (wp⟦x⟧.conjunctive Q₁ Q₂).mpr
